src/coq/AstLib.v
@@ -5,7 +5,6 @@ Require Import Equalities.
 Import ListNotations.
 
 (* Equalities --------------------------------------------------------------- *)
-
 Instance eq_dec_int : eq_dec int := positive_eq_dec.
 
 Module RawID <: UsualDecidableTypeFull.
