src/coq/Effects.v
@@ -1,0 +1,118 @@
+Require Import ZArith List String Omega.
+Require Import  Vellvm.Classes Vellvm.Util.
+Require Import paco.
+Import ListNotations.
+Open Scope positive_scope.
+
+Set Implicit Arguments.
+Set Contextual Implicit.
+
+Module Type EffT.
+  (* The effects interface is parameterized by the language's types and the 
+   memory model's notion of addresses. *)
+  Parameter typ : Set.
+  Parameter addr : Set.
+End EffT.
+
+Module Effects(ET:EffT).
+Export ET.
+  
+(* TODO: Add other memory effects, such as synchronization operations *)
+(* Notes: 
+   - To allow the memory model to correctly model stack alloca deallocation,
+     we would also have to expose the "Ret" instruction. 
+
+   - What is the correct way to model global data? 
+*)
+Inductive effects (dvalue:Type) (d:Type) : Type :=
+| Alloca (t:typ)  (k:dvalue -> d)        (* Stack allocation *)
+| Load   (a:addr) (k:dvalue -> d)
+| Store  (a:addr) (v:dvalue) (k:d)
+| Call   (v:dvalue) (k:dvalue -> d)
+.    
+
+Definition effects_map {A B dvalue} (f:A -> B) (m:effects dvalue A) : effects dvalue B :=
+  match m with
+  | Alloca t g => Alloca t (fun a => f (g a))
+  | Load a g  => Load a (fun dv => f (g dv))
+  | Store a dv d => Store a dv (f d)
+  | Call a d => Call a (fun dv => f (d dv))
+  end.
+
+Instance effects_functor (dvalue:Type) : @Functor (effects dvalue) := fun A => fun B => @effects_map A B dvalue.
+Program Instance effects_functor_eq_laws (dvalue:Type) : (@FunctorLaws (effects dvalue)) (@effects_functor dvalue) (@eq).
+Next Obligation.
+  unfold fmap. unfold effects_functor. unfold effects_map. destruct a; reflexivity.
+Defined.
+Next Obligation.
+  unfold fmap. unfold effects_functor. unfold effects_map. destruct a; reflexivity.
+Defined.  
+
+(* Domain of semantics *)
+CoInductive D dvalue X :=
+| Ret : X -> D dvalue X
+| Fin : D dvalue X
+| Err : D dvalue X 
+| Tau : D dvalue X -> D dvalue X
+| Eff : effects dvalue (D dvalue X) -> D dvalue X
+.
+
+CoFixpoint d_map {A B dvalue} (f:A -> B) (d:D dvalue A) : D dvalue B :=
+  match d with
+    | Ret a => Ret (f a)
+    | Fin => Fin
+    | Err => Err
+    | Tau d' => Tau (d_map f d')
+    | Eff m => Eff (effects_map (d_map f) m)
+  end.
+
+Section UNFOLDING.
+
+Definition id_match_d {A dvalue} (d:D dvalue A) : D dvalue A :=
+  match d with
+    | Ret a => Ret a
+    | Fin => Fin
+    | Err => Err
+    | Tau d' => Tau d'
+    | Eff m => Eff m
+  end.
+
+Lemma id_d_eq : forall A dvalue (d:D dvalue A),
+  d = id_match_d d.
+Proof.
+  destruct d; auto.
+Qed.
+
+End UNFOLDING.
+
+Arguments id_d_eq {_ _} _ .
+
+
+Instance D_functor (dvalue:Type) : @Functor (D dvalue) := fun A => fun B => @d_map A B dvalue.
+
+(* Probably a functor only up to stuttering equivalence. *)
+(*
+Program Instance D_functor_eq_laws : (@FunctorLaws D) D_functor (@eq).
+*)
+
+(* Note: for guardedness, bind Ret introduces extra Tau *)
+Definition bind {A B dvalue} (m:D dvalue A) (f:A -> D dvalue B) : D dvalue B :=
+  (cofix bindf m:= 
+     match m with
+       | Ret a => Tau (f a)
+       | Fin => Fin
+       | Err => Err
+       | Tau d' => Tau (bindf d')
+       | Eff m => Eff (effects_map bindf m)
+     end) m.
+
+Program Instance D_monad (dvalue:Type) : (@Monad (D dvalue)) (@D_functor dvalue) := _.
+Next Obligation.
+  split.
+  - intros. apply Ret. exact X.
+  - intros A B. apply bind.
+Defined.
+  
+Inductive Empty :=.
+
+End Effects.
