src/coq/Extract_Haskell_Ollvm_ast.v
@@ -1,0 +1,15 @@
+Require Import Ascii String.
+Extraction Language Haskell.
+
+Require Import Vellvm.Ollvm_ast.
+
+Extract Inductive option => "Prelude.Maybe" [ "Nothing" "Just" ].
+Extract Inductive list => "[]" [ "[]" "(:)" ].
+Extract Inductive prod => "(,)" [ "(,)" ].
+Extract Inductive string => "Prelude.String" [ "[]" "(:)" ].
+Extract Inductive bool => "Prelude.Bool" [ "False" "True" ].
+Extract Inlined Constant int => "Prelude.Int".
+Extract Inlined Constant float => "Prelude.Float".
+
+Extraction Library Datatypes.
+Extraction Library Ollvm_ast.
