src/coq/Memory.v
@@ -1,0 +1,32 @@
+Require Import ZArith List String Omega.
+Require Import  Vellvm.Ollvm_ast Vellvm.Classes Vellvm.Util.
+Require Import Vellvm.StepSemantics.
+Import ListNotations.
+
+Set Implicit Arguments.
+Set Contextual Implicit.
+
+Module A : Vellvm.StepSemantics.ADDR with Definition addr := nat.
+  Definition addr := nat.
+End A.  
+
+Module SS := StepSemantics.StepSemantics(A).
+Import SS.
+
+Definition mtype := list dvalue.
+Definition undef := DV (VALUE_Undef _).
+
+(* HACK: extract ID_LAZY to lazy to fix broken cofixpoint extraction.  See Memory.ml *)
+Definition ID_LAZY {A:Type} (x:A) := x.
+
+CoFixpoint memD {A} (memory:mtype) (d:Obs A) : Obs A :=
+  match d with
+    | Ret a => ID_LAZY (Ret a)
+    | Fin => ID_LAZY Fin
+    | Err => ID_LAZY Err
+    | Tau d'            => Tau (memD memory d')
+    | Eff (Alloca t k)  => Tau (memD (memory ++ [undef]) (k (DVALUE_Addr (List.length memory))))
+    | Eff (Load a k)    => Tau (memD memory (k (nth_default undef memory a)))
+    | Eff (Store a v k) => Tau (memD (replace memory a v) k)
+    | Eff (Call _ _) => Err
+  end.
