src/coq/Ollvm_ast.v
@@ -1,0 +1,368 @@
+(* {{{ LICENSE                                                              *
+  * vi: set fdm=marker fdl=0:                                                *
+  *                                                                          *
+  * Copyright (c) 2012 Raphaël Proust <raphlalou@gmail.com>                  *
+  * Copyright (c) 2012 INRIA - Raphaël Proust <raphlalou@gmail.com>          *
+  * Copyright (c) 2012 ENS - Raphaël Proust <raphlalou@gmail.com>            *
+  * Copyright (c) 2014 OCamlPro - Julien Sagot <ju.sagot@gmail.com>          *
+  *                                                                          *
+  * Permission to use, copy, modify, and distribute this software for any    *
+  * purpose with or without fee is hereby granted, provided that the above   *
+  * copyright notice and this permission notice appear in all copies.        *
+  *                                                                          *
+  * THE SOFTWARE IS PROVIDED "AS IS" AND THE AUTHOR DISCLAIMS ALL WARRANTIES *
+  * WITH REGARD TO THIS SOFTWARE INCLUDING ALL IMPLIED WARRANTIES OF         *
+  * MERCHANTABILITY AND FITNESS. IN NO EVENT SHALL THE AUTHOR BE LIABLE FOR  *
+  * ANY SPECIAL, DIRECT, INDIRECT, OR CONSEQUENTIAL DAMAGES OR ANY DAMAGES   *
+  * WHATSOEVER RESULTING FROM LOSS OF USE, DATA OR PROFITS, WHETHER IN AN    *
+  * ACTION OF CONTRACT, NEGLIGENCE OR OTHER TORTIOUS ACTION, ARISING OUT OF  *
+  * OR IN CONNECTION WITH THE USE OR PERFORMANCE OF THIS SOFTWARE.           *
+  * }}}                                                                      
+
+  Ported from ollvm_ast.ml
+  Copyright (c) 2016 Steve Zdancewic <stevez@cis.upenn.edu>
+*)
+
+Require Import List. 
+Require Import String Ascii.
+Require Import ZArith.ZArith_base.
+Open Scope string_scope.
+Open Scope list_scope.
+
+
+Definition int := positive.
+Parameter float : Set.
+
+Inductive linkage : Set :=
+| LINKAGE_Private
+| LINKAGE_Internal
+| LINKAGE_Available_externally
+| LINKAGE_Linkonce
+| LINKAGE_Weak
+| LINKAGE_Common
+| LINKAGE_Appending
+| LINKAGE_Extern_weak
+| LINKAGE_Linkonce_odr
+| LINKAGE_Weak_odr
+| LINKAGE_External
+.
+      
+Inductive dll_storage : Set :=
+| DLLSTORAGE_Dllimport
+| DLLSTORAGE_Dllexport
+.      
+
+Inductive visibility : Set :=
+| VISIBILITY_Default
+| VISIBILITY_Hidden
+| VISIBILITY_Protected
+.
+    
+Inductive cconv : Set :=
+| CC_Ccc
+| CC_Fastcc
+| CC_Coldcc
+| CC_Cc (cc:int)
+.
+        
+Inductive param_attr : Set :=
+| PARAMATTR_Zeroext
+| PARAMATTR_Signext
+| PARAMATTR_Inreg
+| PARAMATTR_Byval
+| PARAMATTR_Inalloca
+| PARAMATTR_Sret
+| PARAMATTR_Align (a:int)
+| PARAMATTR_Noalias
+| PARAMATTR_Nocapture
+| PARAMATTR_Nest
+| PARAMATTR_Returned
+| PARAMATTR_Nonnull
+| PARAMATTR_Dereferenceable (a:int)
+.
+                            
+Inductive fn_attr : Set :=
+| FNATTR_Alignstack (a:int)
+| FNATTR_Alwaysinline
+| FNATTR_Builtin
+| FNATTR_Cold
+| FNATTR_Inlinehint
+| FNATTR_Jumptable
+| FNATTR_Minsize
+| FNATTR_Naked
+| FNATTR_Nobuiltin
+| FNATTR_Noduplicate
+| FNATTR_Noimplicitfloat
+| FNATTR_Noinline
+| FNATTR_Nonlazybind
+| FNATTR_Noredzone
+| FNATTR_Noreturn
+| FNATTR_Nounwind
+| FNATTR_Optnone
+| FNATTR_Optsize
+| FNATTR_Readnone
+| FNATTR_Readonly
+| FNATTR_Returns_twice
+| FNATTR_Sanitize_address
+| FNATTR_Sanitize_memory
+| FNATTR_Sanitize_thread
+| FNATTR_Ssp
+| FNATTR_Sspreq
+| FNATTR_Sspstrong
+| FNATTR_Uwtable
+| FNATTR_String (s:string) (* "no-see" *)
+| FNATTR_Key_value (kv : string * string) (* "unsafe-fp-math"="false" *)
+| FNATTR_Attr_grp (g:int)
+.
+
+
+Inductive raw_id : Set :=
+| Name (s:string)     (* Named identifiers are strings: %argc, %val, %x, @foo, @bar etc. *)  
+| Anon (n:int)        (* Anonymous identifiers must be sequentially numbered %0, %1, %2, etc. *)
+.
+
+Inductive ident : Set :=
+| ID_Global (id:raw_id)   (* @id *)
+| ID_Local  (id:raw_id)   (* %id *)
+.
+
+(* auxilliary definitions for when we know which case we're in already *)
+Definition local_id  := raw_id.
+Definition global_id := raw_id.
+
+Definition function_id := global_id.
+Definition block_id := local_id.
+
+Inductive typ : Set :=
+| TYPE_I (sz:int)
+| TYPE_Pointer (t:typ)
+| TYPE_Void
+| TYPE_Half
+| TYPE_Float
+| TYPE_Double
+| TYPE_X86_fp80
+| TYPE_Fp128
+| TYPE_Ppc_fp128
+| TYPE_Label
+| TYPE_Metadata
+| TYPE_X86_mmx
+| TYPE_Array (sz:int) (t:typ)
+| TYPE_Function (ret:typ) (args:list typ)
+| TYPE_Struct (fields:list typ)
+| TYPE_Packed_struct (fields:list typ)
+| TYPE_Opaque
+| TYPE_Vector (sz:int) (t:typ)
+| TYPE_Identified (id:ident)
+.
+
+
+Inductive icmp : Set := Eq|Ne|Ugt|Uge|Ult|Ule|Sgt|Sge|Slt|Sle.
+Inductive fcmp : Set := FFalse|FOeq|FOgt|FOge|FOlt|FOle|FOne|FOrd|FUno|FUeq|FUgt|FUge|FUlt|FUle|FUne|FTrue.
+
+
+Inductive ibinop : Set :=
+| Add (nuw:bool) (nsw:bool)
+| Sub (nuw:bool) (nsw:bool)
+| Mul (nuw:bool) (nsw:bool)
+| Shl (nuw:bool) (nsw:bool)
+| UDiv (exact:bool)
+| SDiv (exact:bool)
+| LShr (exact:bool)
+| AShr (exact:bool)
+| URem | SRem | And | Or | Xor
+.
+
+Inductive fbinop : Set :=
+  FAdd | FSub | FMul | FDiv | FRem.
+
+Inductive fast_math : Set :=
+  Nnan | Ninf | Nsz | Arcp | Fast.
+
+Inductive conversion_type : Set :=
+  Trunc | Zext | Sext | Fptrunc | Fpext | Uitofp | Sitofp | Fptoui |
+  Fptosi | Inttoptr | Ptrtoint | Bitcast.
+
+Definition tident : Set := (typ * ident)%type.
+
+
+(* NOTES: 
+
+  This is the "functorial" presentation of the syntax.  Note that the 'value' type 
+  declared below actually creates the fixpoint.  Setting things up this way means 
+  that we can re-use this functor for defining the dynamic values (over in
+  StepSemantics.v) but we have to do some work to define appropriate induction
+  principles (see AstInd.v).
+
+  This datatype is more permissive than legal in LLVM:
+     - it allows identifiers to appear nested inside of "constant expressions"
+
+  NOTES:
+   Integer values: llc parses large integer values and converts them to some 
+   internal form (based on integer size?)
+   
+   Why do we need Bool?  Why not i1 ?  Is that "real" llvm?
+ *)
+Inductive Expr (a:Set) : Set :=
+| VALUE_Ident   (id:ident)  
+| VALUE_Integer (x:int)
+| VALUE_Float   (f:float)
+| VALUE_Bool    (b:bool)
+| VALUE_Null
+| VALUE_Zero_initializer
+| VALUE_Cstring (s:string)
+| VALUE_None                                       (* "token" constant *)
+| VALUE_Undef
+| VALUE_Struct        (fields: list (typ * a))
+| VALUE_Packed_struct (fields: list (typ * a))
+| VALUE_Array         (elts: list (typ * a))
+| VALUE_Vector        (elts: list (typ * a))
+| OP_IBinop           (iop:ibinop) (t:typ) (v1:a) (v2:a)  
+| OP_ICmp             (cmp:icmp)   (t:typ) (v1:a) (v2:a)
+| OP_FBinop           (fop:fbinop) (fm:list fast_math) (t:typ) (v1:a) (v2:a)
+| OP_FCmp             (cmp:fcmp)   (t:typ) (v1:a) (v2:a)
+| OP_Conversion       (conv:conversion_type) (t_from:typ) (v:a) (t_to:typ)
+| OP_GetElementPtr    (t:typ) (ptrval:(typ * a)) (idxs:list (typ * a))
+| OP_ExtractElement   (vec:(typ * a)) (idx:(typ * a))
+| OP_InsertElement    (vec:(typ * a)) (elt:(typ * a)) (idx:(typ * a))
+| OP_ShuffleVector    (vec1:(typ * a)) (vec2:(typ * a)) (idxmask:(typ * a))
+| OP_ExtractValue     (vec:(typ * a)) (idxs:list int)
+| OP_InsertValue      (vec:(typ * a)) (elt:(typ * a)) (idxs:list int)
+| OP_Select           (cnd:(typ * a)) (v1:(typ * a)) (v2:(typ * a)) (* if * then * else *)
+.
+
+(* static values *)
+Inductive value : Set :=
+| SV : Expr value -> value.
+            
+Definition tvalue : Set := typ * value.
+
+Inductive instr_id : Set :=
+| IId   (id:raw_id)    (* "Anonymous" or explicitly named instructions *)
+| IVoid (n:int)        (* "Void" return type, for "store" "call" and terminators.
+                           Each with unique number (NOTE: these are distinct from Anon raw_id) *)
+.
+        
+Inductive instr : Set :=
+| INSTR_Op   (op:value)                          (* INVARIANT: op must be of the form SV (OP_ ...) *)
+| INSTR_Call (fn:tident) (args:list tvalue)      (* CORNER CASE: return type is void treated specially *)
+
+| INSTR_Phi  (t:typ) (args:list (ident * value))
+
+| INSTR_Alloca (t:typ) (nb: option tvalue) (align:option int) 
+| INSTR_Load  (volatile:bool) (t:typ) (ptr:tvalue) (align:option int)       
+| INSTR_Store (volatile:bool) (val:tvalue) (ptr:tvalue) (align:option int)
+| INSTR_Fence
+| INSTR_AtomicCmpXchg
+| INSTR_AtomicRMW
+| INSTR_Unreachable
+
+| INSTR_VAArg
+| INSTR_LandingPad
+.
+
+Inductive terminator : Set :=
+(* Terminators *)
+(* Types in branches are TYPE_Label constant *)
+| TERM_Ret        (v:tvalue)
+| TERM_Ret_void
+| TERM_Br         (v:tvalue) (br1:tident) (br2:tident) 
+| TERM_Br_1       (br:tident)
+| TERM_Switch     (v:tvalue) (default_dest:tident) (brs: list (tvalue * tident))
+| TERM_IndirectBr (v:tvalue) (brs:list tident) (* address * possible addresses (labels) *)
+| TERM_Resume     (v:tvalue)
+| TERM_Invoke     (fnptrval:tident) (args:list tvalue) (to_label:tident) (unwind_label:tident)
+.
+
+Inductive thread_local_storage : Set :=
+| TLS_Localdynamic
+| TLS_Initialexec
+| TLS_Localexec
+.
+
+Record global : Set :=
+  mk_global {
+      g_ident        : global_id;
+      g_typ          : typ;
+      g_constant     : bool;
+      g_value        : option value;
+
+      g_linkage      : option linkage;
+      g_visibility   : option visibility;
+      g_dll_storage  : option dll_storage;
+      g_thread_local : option thread_local_storage;
+      g_unnamed_addr : bool;
+      g_addrspace    : option int;
+      g_externally_initialized: bool;
+      g_section      : option string;
+      g_align        : option int;
+}.
+
+Record declaration : Set :=
+  mk_declaration
+  {
+    dc_name        : function_id;  
+    dc_type        : typ;    (* INVARIANT: should be TYPE_Function (ret_t * args_t) *)
+    dc_param_attrs : list param_attr * list (list param_attr); (* ret_attrs * args_attrs *)
+    dc_linkage     : option linkage;
+    dc_visibility  : option visibility;
+    dc_dll_storage : option dll_storage;
+    dc_cconv       : option cconv;
+    dc_attrs       : list fn_attr;
+    dc_section     : option string;
+    dc_align       : option int;
+    dc_gc          : option string;
+  }.
+
+
+
+Record block : Set :=
+  mk_block
+    {
+      blk_id      : block_id;
+      blk_instrs  : list (instr_id * instr);
+      blk_term    : terminator;
+      blk_term_id : instr_id;      
+    }.
+
+Record definition :=
+  mk_definition
+  {
+    df_prototype   : declaration;
+    df_args        : list local_id;
+    df_instrs      : list block;
+  }.
+
+Inductive metadata : Set :=
+  | METADATA_Const  (tv:tvalue)
+  | METADATA_Null
+  | METADATA_Id     (id:raw_id)  (* local or global? *)
+  | METADATA_String (str:string)
+  | METADATA_Named  (strs:list string)
+  | METADATA_Node   (mds:list metadata)
+.
+
+Inductive toplevel_entity : Set :=
+| TLE_Target          (tgt:string)
+| TLE_Datalayout      (layout:string)
+| TLE_Declaration     (decl:declaration)
+| TLE_Definition      (defn:definition)
+| TLE_Type_decl       (id:ident) (t:typ)
+| TLE_Source_filename (s:string)
+| TLE_Global          (g:global)
+| TLE_Metadata        (id:raw_id) (md:metadata)
+| TLE_Attribute_group (i:int) (attrs:list fn_attr)
+.
+
+Record modul : Set :=
+  mk_modul
+  {
+    m_name: string;
+    m_target: toplevel_entity;
+    m_datalayout: toplevel_entity;
+    m_globals: list (string * global);
+    m_declarations: list (string * declaration);
+    m_definitions: list (string * definition);
+  }.
+
+
+Definition toplevel_entities : Set := list toplevel_entity.
