src/ml/extracted/Extract.v
@@ -1,0 +1,42 @@
+Require Vellvm.Ollvm_ast.
+Require Vellvm.Transform.
+Require Vellvm.Memory.
+
+Require ExtrOcamlBasic.
+Require ExtrOcamlString.
+Require ExtrOcamlIntConv.
+
+Extraction Language Ocaml.
+Extraction Blacklist String List.
+
+
+(* strings ------------------------------------------------------------------ *)
+(*
+Extract Inductive ascii => char
+[
+"(* If this appears, you're using Ascii internals. Please don't *) (fun (b0,b1,b2,b3,b4,b5,b6,b7) -> let f b i = if b then 1 lsl i else 0 in Char.chr (f b0 0 + f b1 1 + f b2 2 + f b3 3 + f b4 4 + f b5 5 + f b6 6 + f b7 7))"
+]
+"(* If this appears, you're using Ascii internals. Please don't *) (fun f c -> let n = Char.code c in let h i = (n land (1 lsl i)) <> 0 in f (h 0) (h 1) (h 2) (h 3) (h 4) (h 5) (h 6) (h 7))".
+
+Extract Constant zero => "'\000'".
+Extract Constant one => "'\001'".
+Extract Constant shift =>
+ "fun b c -> Char.chr (((Char.code c) lsl 1) land 255 + if b then 1 else 0)".
+
+Extract Inlined Constant ascii_dec => "(=)".
+Extract Inductive string => "string" [ "str_nil" "str_cons" ].
+*)
+
+(* OCaml pervasive types ---------------------------------------------------- *)
+Extract Inlined Constant Ollvm_ast.int => "int".
+Extract Inlined Constant Ollvm_ast.float => "float".
+
+Extract Inlined Constant Memory.ID_LAZY => "lazy".
+
+Set Extraction AccessOpaque.
+(* NOTE: assumes that this file is compiled from /src *)
+Cd "ml/extracted".
+
+Extraction Library ExtrOcamlIntConv.
+Recursive Extraction Library Memory.
+Extraction Library Transform.
